finish the proof of the AggregatingProgram compiler

src/datalog/AggregatingProgram.v
@@ -98,6 +98,10 @@ Section well_formed.
     wf_Sexpr ctx _ (bop_over_set o x1) (bop_over_set o x2).
 End well_formed.
 
+Definition SExpr t := forall var, Sexpr var t.
+Definition Wf_Sexpr {t} (e : SExpr t) :=
+  forall var1 var2, wf_Sexpr [] t (e var1) (e var2).
+
 Definition lit x : expr := fun_expr (fn_lit x) [].
 
 Definition interp_bop o x y :=
@@ -411,29 +415,52 @@ Ltac destr_vbp :=
         specialize (H (fun _ => False))
     end.
 
+Lemma vars_in_incl var (ctx1 ctx2 : list var) (p : blocks_prog var) :
+  incl ctx1 ctx2 ->
+  vars_in ctx1 p ->
+  vars_in ctx2 p.
+Proof.
+  intros Hincl Hvars. revert ctx2 Hincl.
+  induction Hvars; intros; constructor; auto with incl.
+  eapply Forall_impl; [|eassumption]. intros [? ?]. auto with incl.
+Qed.
+Hint Resolve vars_in_incl : core.
+
 Hint Constructors vars_in : core.
-Lemma compile_Sexpr_honest_args var1 var2 t e (ctx : list (@ctx_elt2 var1 (fun _ => var2))) e0 :
+Lemma compile_Sexpr_vars_in var1 var2 t (dummy : forall t, var1 t) e (ctx : list (@ctx_elt2 var1 (fun _ => var2))) e0 :
   wf_Sexpr ctx t e e0 ->
   vars_in (map (@ctx_elt_p2 _ (fun _ => _)) ctx) (compile_Sexpr e0).
 Proof.
-  induction 1; simpl; eauto.
-  - constructor. constructor; eauto. apply in_map_iff. eauto. eexists.
-    split; [|eassumption]. reflexivity.
-  - constructor; eauto. intros. constructor; eauto. 1: admit.
-    intros. constructor; eauto. constructor; simpl; eauto.
-  - constructor; eauto. intros. constructor; eauto. 1: admit.
-    intros. constructor; eauto.
-Abort.
+  induction 1;
+    repeat match goal with
+      | _ => progress (intros; simpl in * )
+      | |- vars_in _ _ => constructor
+      | |- In _ (map _ _) => apply in_map_iff
+      | |- Forall _ (_ :: _) => constructor
+      | |- Forall _ [] => constructor
+      | _ => solve[eauto]
+      | |- vars_in (_ :: _) _ => eapply vars_in_incl; [|solve[eauto]]; auto with incl
+      end.
+  eexists. split; [|eassumption]. reflexivity.
+Qed.
+
+Definition dummy (t : type) : interp_type t :=
+  match t with
+  | val => O
+  | set => fun _ => False
+  end.
+Hint Resolve dummy : core.
 
 Hint Unfold Option.option_relation : core.
 Lemma compile_Sexpr_correct ctx t e e0 e' :
   wf_Sexpr ctx t e e0 ->
   Forall (fun elt => agrees elt.(ctx_elt_p2) elt.(ctx_elt_p1)) ctx ->
+  Forall honest_args (map (@ctx_elt_p2 _ (fun _ => _)) ctx) ->
   valid_blocks_prog (compile_Sexpr e0) ->
   interp_Sexpr e e' ->
   agrees (interp_blocks_prog (compile_Sexpr e0)) e'.
 Proof.
-  intros Hwf Hctx Hnl. revert e'. induction Hwf; intros e' He'.
+  intros Hwf Hctx Hhonest Hvalid. revert e'. induction Hwf; intros e' He'.
   - dep_invert He'. rewrite Forall_forall in Hctx.
     specialize (Hctx _ H). clear H. simpl in Hctx.
     cbv [agrees] in Hctx. fwd. cbv [agrees]. simpl. split.
@@ -450,8 +477,8 @@ Proof.
       -- interp_exprs.
   - dep_invert He'.
     destr_vbp.
-    specialize (IHHwf1 ltac:(eassumption) ltac:(eassumption) _ ltac:(eassumption)).
-    specialize (IHHwf2 ltac:(eassumption) ltac:(eassumption) _ ltac:(eassumption)).
+    specialize (IHHwf1 ltac:(eassumption) ltac:(eassumption) ltac:(eassumption) _ ltac:(eassumption)).
+    specialize (IHHwf2 ltac:(eassumption) ltac:(eassumption) ltac:(eassumption) _ ltac:(eassumption)).
     cbv [agrees] in IHHwf1, IHHwf2. fwd.
     simpl. split.
     + intros x. simpl. split.
@@ -482,14 +509,14 @@ Proof.
          eapply meta_rule_impl with (ctx := map.empty) (S := fun _ => _); interp_exprs.
       -- interp_exprs.
   - dep_invert He'.
-    specialize (IHHwf ltac:(eassumption) ltac:(eassumption) _ ltac:(eassumption)).
+    specialize (IHHwf ltac:(eassumption) ltac:(eassumption) ltac:(eassumption) _ ltac:(eassumption)).
     cbv [agrees] in IHHwf. fwd. split.
     + intros x. rewrite <- IHHwfp0. split; auto.
     + eauto.
   - dep_invert He'.
     destr_vbp.
-    specialize (IHHwf1 ltac:(eassumption) ltac:(eassumption) _ ltac:(eassumption)).
-    specialize (IHHwf2 ltac:(eassumption) ltac:(eassumption) _ ltac:(eassumption)).
+    specialize (IHHwf1 ltac:(eassumption) ltac:(eassumption) ltac:(eassumption) _ ltac:(eassumption)).
+    specialize (IHHwf2 ltac:(eassumption) ltac:(eassumption) ltac:(eassumption) _ ltac:(eassumption)).
     cbv [agrees] in IHHwf1, IHHwf2. cbv [agrees]. fwd. simpl. split.
     + intros x. rewrite IHHwf1p0, IHHwf2p0. clear IHHwf1p0 IHHwf2p0. split.
       -- intros [? ?]. eapply prog_impl_step.
@@ -503,9 +530,14 @@ Proof.
       -- interp_exprs.
   - rename H0 into IHHwf'.
     dep_invert He'.
-    simpl in Hnl. fwd.
-    specialize (IHHwf ltac:(eassumption) ltac:(eassumption) _ ltac:(eassumption)).
-    specialize (IHHwf' _ _ ltac:(eauto) ltac:(eauto) _ ltac:(eauto)).
+    simpl in Hvalid. fwd.
+    specialize (IHHwf ltac:(eassumption) ltac:(eassumption) ltac:(eassumption) _ ltac:(eassumption)).
+    simpl in IHHwf'.
+    epose_dep IHHwf'.
+    specialize (IHHwf' ltac:(eauto)). specialize' IHHwf'.
+    { constructor; auto. eapply interp_blocks_prog_honest; eauto.
+      eapply compile_Sexpr_vars_in; eauto. }
+    specialize (IHHwf' ltac:(eauto) ltac:(eauto) ltac:(eauto)).
     clear Hctx. cbv [agrees] in *. fwd. split.
     + intros x. rewrite IHHwf'p0. clear IHHwf'p0.
       simpl. reflexivity.
@@ -513,7 +545,7 @@ Proof.
   - dep_invert He'.
     destr_vbp.
     rename H2 into Hset.
-    specialize (IHHwf ltac:(eassumption) ltac:(eassumption) _ ltac:(eassumption)).
+    specialize (IHHwf ltac:(eassumption) ltac:(eassumption) ltac:(eassumption) _ ltac:(eassumption)).
     cbv [agrees]. simpl. cbv [agrees] in IHHwf. fwd. split.
     + intros x. split.
       -- intros. subst. eapply prog_impl_step.
@@ -539,54 +571,57 @@ Proof.
                 ---- simpl. constructor; [|constructor]. apply prog_impl_leaf.
                      simpl. doExists 0. split; [reflexivity|].
                      eapply use_valid_blocks_prog; [eauto|eauto|idtac|eauto].
-
-
-                (*TODO continue here; instead of using wf_blah should have some
-                 simpler predicate that says something about all variables
-                 in the program satisfying some property*)
-
-
+                     ++++ eapply compile_Sexpr_vars_in. 2: eassumption. 1: eauto.
+                     ++++ eassumption.
             +++ simpl. intros. repeat invert_stuff. split.
-                ---- intros H. cbv [one_step_derives one_step_derives0] in H. fwd. repeat invert_stuff.
-                     eexists. split; [reflexivity|]. apply IHHwfp0.
-                     cbv [fact_supported] in H4. repeat invert_stuff.
-                     simpl in H0. destruct H0; try contradiction.
-                     cbv [fact_matches] in H. repeat invert_stuff.
-
-
-                     Search valid_blocks_prog.
-                     eapply interp_blocks_prog_honest
-                     Check compile_Sexpr.
-                     simpl in H.
-                     Search y. Search y. assumption.
-                ---- intros H. fwd.
-                    eapply block_prog_impl_step.
-                    ++++ simpl. do 2 apply Exists_cons_tl. apply Exists_cons_hd.
-                         constructor.
-                         eapply normal_rule_impl with (ctx := map.put map.empty 0 _); interp_exprs.
-                    ++++ interp_exprs. apply IHHwfp0. assumption.
-         --- rewrite map_map. apply Forall_map.
-            cbv [is_list_set] in Hset. fwd. apply Forall_forall.
-            intros x Hx. apply Hsetp0 in Hx. apply IHHwfp0 in Hx.
-            eapply block_prog_impl_step.
-            +++ simpl. do 2 apply Exists_cons_tl. apply Exists_cons_hd.
-                constructor.
-                eapply normal_rule_impl with (ctx := map.put map.empty 0 _); interp_exprs.
-            +++ interp_exprs.
-      -- intros H. Print honest_block_prog.
+                ---- intros H. repeat invert_stuff.
+                     eexists. split; [reflexivity|]. apply IHHwfp0. assumption.
+                ---- intros H. fwd. cbv [one_step_derives one_step_derives0].
+                     eexists. split.
+                     { doExists 2.
+                       eapply normal_rule_impl with (ctx := map.put map.empty 0 _); interp_exprs. }
+                     interp_exprs. cbv [fact_supported]. doExists 0. simpl.
+                     right.
+                     (*TODO maybe this should work?*) Fail solve [interp_exprs].
+                     cbv [fact_matches]. do 4 eexists. ssplit; eauto. interp_exprs.
+            +++ simpl. intros H. repeat invert_stuff.
+            --- rewrite map_map. apply Forall_map.
+                cbv [is_list_set] in Hset. fwd. apply Forall_forall.
+                intros x Hx. apply Hsetp0 in Hx. apply IHHwfp0 in Hx.
+                eapply prog_impl_step.
+                +++ simpl. doExists 2. constructor.
+                    eapply normal_rule_impl with (ctx := map.put map.empty 0 _); interp_exprs.
+                +++ interp_exprs.
+      -- intros H.
          repeat lazymatch goal with
-                | H: block_prog_impl _ _ (meta_fact _ _ _) |- _ => fail
+                | H: prog_impl _ _ (meta_fact _ _ _) |- _ => fail
                 | _ => invert_stuff
                 end.
          lazymatch goal with
-         | H: block_prog_impl _ _ (meta_fact _ _ _) |- _ => rename H into Hmf
+         | H: prog_impl _ _ (meta_fact _ _ _) |- _ => rename H into Hmf
          end.
-         apply Hnlp1 in Hmf. move Hmf at bottom.
+         simpl in Hvalidp1. fwd.
+         apply valid_impl_honest in Hvalidp1p0.
+         apply Hvalidp1p0 in Hmf.
+         2: { cbv [good_inputs]. simpl. split.
+              - intros ? ? ?. repeat invert_stuff.
+                destruct f; simpl in *; subst;
+                (*TODO should not do this*)
+                  repeat match goal with
+                    | H0 : _ \/ _ |- _ => destruct H0 as [H0|H0]; [rewrite <- H0 in *; congruence|]
+                    end;
+                  contradiction.
+              - cbv [doesnt_lie]. intros. repeat invert_stuff.
+                eapply interp_blocks_prog_honest in H2p1; eauto.
+                2: { eapply compile_Sexpr_vars_in; eauto. }
+                cbv [consistent]. intros. cbv [args_consistent] in H2p1.
+                rewrite H2p1 by assumption. split; intros; repeat invert_stuff; eauto. }
+         move Hmf at bottom.
          assert (Heq: forall x y, (x = y /\ x' x) <-> S0 [x; y]).
          { intros x y. cbv [consistent] in Hmf. rewrite Hmf; [|interp_exprs].
            rewrite IHHwfp0. split.
-           - intros H. fwd. eapply block_prog_impl_step.
-             + simpl. do 2 apply Exists_cons_tl. apply Exists_cons_hd. constructor.
+           - intros H. fwd. eapply prog_impl_step.
+             + simpl. doExists 2. constructor.
                eapply normal_rule_impl with (ctx := map.put map.empty 0 _); interp_exprs.
              + interp_exprs.
            - intros H. repeat invert_stuff. auto. }
@@ -608,13 +643,27 @@ Proof.
          apply FinFun.Injective_map_NoDup_in; [|assumption].
          intros (?, ?) (?, ?). simpl. intros H1' H2' ?. subst.
          apply Hset'p0 in H1', H2'. apply Heq in H1', H2'. fwd. reflexivity.
-    + eexists. eapply block_prog_impl_step.
-      -- simpl. apply Exists_cons_tl. apply Exists_cons_hd.
+    + eexists. eapply prog_impl_step.
+      -- simpl. doExists 1.
          eapply meta_rule_impl with (ctx := map.empty) (S := fun _ => _); interp_exprs.
-      -- interp_exprs. eapply block_prog_impl_step.
-         ++ simpl. do 3 apply Exists_cons_tl. apply Exists_cons_hd.
+      -- interp_exprs. eapply prog_impl_step.
+         ++ simpl. doExists 3.
             eapply meta_rule_impl with (ctx := map.empty) (S := fun _ => _); interp_exprs.
          ++ interp_exprs.
             Unshelve.
             all: exact True.
+Qed.
+
+Lemma compile_SExpr_correct t (e : SExpr t) e' :
+  Wf_Sexpr e ->
+  interp_Sexpr (e _) e' ->
+  agrees (interp_blocks_prog (compile_Sexpr (e _))) e'.
+Proof.
+  intros Hwf Hinterp.
+  eapply compile_Sexpr_correct with (ctx := []).
+  - apply Hwf.
+  - constructor.
+  - constructor.
+  - apply compile_Sexpr_valid.
+  - exact Hinterp.
 Qed.
